src/common/Nemonuri.IndexSet.fst
@@ -1,35 +1,41 @@
 module Nemonuri.IndexSet
 
 module I = FStar.IntegerIntervals
-module FSet = FStar.FiniteSet.Base
-open FStar.FiniteSet.Ambient
+module Set = FStar.Set
+
+(* Node:
+   'Set' 은 '구성(Construction) 가능한 술어(Predicate)'로,
+   'Map' 은 '구성 가능한 함수'로 생각할 수 있다.
+*)
 
 noeq
 type unrefined_t = {
   count: nat;
-  set: FSet.set int
+  set: Set.set int
 }
 
 let index_set_predicate (s:unrefined_t) =
-  forall (x:int). (I.interval_condition 0 s.count x) <==> (FSet.mem x s.set)
+  forall (x:int). ((Set.mem x s.set) <==> (I.interval_condition 0 s.count x))
 
 type t = x:unrefined_t{index_set_predicate x}
 
+let mem (s:t) (x:int) : Tot bool = Set.mem x s.set
+
 let empty : t = {
-  count = 0; set = FSet.emptyset #int
+  count = 0; set = Set.empty #int
 }
 
 let push (s:t) : Tot t =
   {
     count = s.count + 1;
-    set = FSet.insert s.count s.set
+    set = Set.add s.count s.set
   }
 
 let pop (s:t{s.count > 0}) : Tot (t & nat) =
   let popped = s.count - 1 in
   let next_set = {
     count = popped;
-    set = FSet.remove popped s.set
+    set = Set.remove popped s.set
   } in
   (next_set, popped)
 
@@ -41,3 +47,4 @@ let rec push_many (s:t) (n:nat)
 
 let create (n:nat) : Tot t =
   push_many empty n
+
